\documentclass[10pt,a4paper]{article}
\usepackage[utf8]{inputenc}
\usepackage[german]{babel}
\usepackage{mathrsfs}
\usepackage{amsmath}
\usepackage{amsfonts}
\usepackage{amssymb}
\usepackage{amsthm}
\usepackage[left=2cm,right=2cm,top=2cm,bottom=2cm]{geometry}

\begin{document}

\section{Aufgabe 1}

\begin{equation}
  p(M) = 0.1, p(m) = 0.02, p(e) = 0.88, p(n | M) = 0.99, p(n | m) = 0.3, p(n | e) = 0.1
\end{equation}

\begin{align*}
  p(M | n) & = \frac{p(n | M) \cdot p(M)}{p(n)}\\
  & = \frac{p(n | M) \cdot p(M)}{p(n | M) + p(n | m) + p(n | e)}\\
  & \simeq 0.071223
\end{align*}

\section{Aufgabe 2}

\subsection{Teil a}

Das ist direkt gegeben.

\subsection{Teil b}

\begin{align*}
  p(B | \lnot A) & = \frac{p(\lnot A | B) \cdot p(B)}{p(\lnot A)}\\
  & = \frac{(1 - p(A | B)) \cdot p(B)}{p(\lnot A)}\\
  & = \frac{(1 - \frac{p(B | A) \cdot p(A)}{p(B)}) \cdot p(B)}{p(\lnot A)}\\
  & \le \frac{(1 - \frac{p(B) \cdot p(A)}{p(B)}) \cdot p(B)}{p(\lnot A)}\\
  & = \frac{(1 - p(A)) \cdot p(B)}{p(\lnot A)}\\
  & = \frac{p(\lnot A) \cdot p(B)}{p(\lnot A)}\\
  & = p(B)
\end{align*}

\subsection{Teil c}

\begin{align*}
  p(A | B) & = \frac{p(B | A) \cdot p(A)}{p(B)}\\
  & \ge \frac{p(B) \cdot p(A)}{p(B)} = p(A)
\end{align*}

\subsection{Teil d}

\begin{align*}
  p(A | \lnot B) & = \frac{p(\lnot B | A) \cdot p(A)}{p(\lnot B)}\\
  & = \frac{(1 - p(B | A)) \cdot p(A)}{p(\lnot B)}\\
  & \le \frac{(1 - p(B)) \cdot p(A)}{p(\lnot B)}\\
  & = \frac{p(\lnot B) \cdot p(A)}{p(\lnot B)}\\
  & = p(A)
\end{align*}

\section{Aufgabe 3}

\begin{equation}
  A = \textit{Hat Brustkrebs}
\end{equation}
\begin{equation}
  B = \textit{Hat ein positives Mammogramm}
\end{equation}
\begin{equation}
  p(A) = 0.008, p(B | A) = 0.9, p(B | \lnot A) = 0.07
\end{equation}
\begin{align*}
  p(A | B) & = \frac{p(B | A) \cdot p(A)}{p(B)}\\
  & = \frac{p(B | A) \cdot p(A)}{p(B | A) \cdot p(A) + p(B | \lnot A) \cdot p(\lnot A)}\\
  & = \frac{p(B | A) \cdot p(A)}{p(B | A) \cdot p(A) + p(B | \lnot A) \cdot (1 - p(A))}\\
  & = \frac{0.9 \cdot 0.008}{0.9 \cdot 0.008 + 0.07 \cdot (1 - 0.008)} \simeq 0.09395
\end{align*}

\section{Aufgabe 4}

\begin{equation}
  \lambda = \textit{Gefangener $\lambda$ ist begnadigt}, \lambda \in \{ A, B, C \}
\end{equation}
\begin{equation}
  W_{\lambda} = \textit{WÃ¤rter sagt $\lambda$}, \lambda \in \{ A, B, C \}
\end{equation}
\begin{equation}
  p(\lambda) = \frac{1}{3}, \lambda \in \{ A, B, C \}
\end{equation}
\begin{equation}
  p(W_{C} | B) = 1, p(W_{B} | C) = 1, p(W_{B} | A) = p(W_{C} | A) = \frac{1}{2}
\end{equation}
\begin{align*}
  p(W_{B}) & = p(W_{B} | A) \cdot p(A) + p(W_{B} | B) \cdot p(B) + p(W_{B} | C) \cdot p(C)\\
  & = \frac{1}{3} \cdot \left( \frac{1}{2} + 1 + 0 \right) = \frac{1}{2}
\end{align*}
\begin{align*}
  p(A | W_{B}) & = \frac{p(W_{B} | A) \cdot p(A)}{p(W_{B})}\\
  & = \frac{\frac{1}{2} \cdot \frac{1}{3}}{\frac{1}{2}} = \frac{1}{3}
\end{align*}
\begin{align*}
  p(C | W_{B}) & = \frac{p(W_{B} | C) \cdot p(C)}{p(W_{B})}\\
  & = \frac{1 \cdot \frac{1}{3}}{\frac{1}{2}} = \frac{2}{3}
\end{align*}
C hat Recht.

\end{document}