\documentclass[10pt,a4paper]{article}
\usepackage[utf8]{inputenc}
\usepackage[german]{babel}
\usepackage{mathrsfs}
\usepackage{amsmath}
\usepackage{amsfonts}
\usepackage{amssymb}
\usepackage{amsthm}
\usepackage[left=2cm,right=2cm,top=2cm,bottom=2cm]{geometry}

\begin{document}

\section{Aufgabe 21}

\subsection{Teil a}

Man f√ºhrt die Rombergapproximation des Integrals mit den gegebenen $a, b$ durch.
\begin{equation}
  I_{1, 1} = \frac{b - a}{2}(f(a) + f(b)) = h(f(a) + f(b))
\end{equation}
\begin{equation}
  I_{2, 1} = \frac{b - a}{4}(f(a) + f(b) + 2f(a + \frac{b - a}{2})) = \frac{h}{2}(f(a) + f(b) + 2f(\frac{a + b}{2}))
\end{equation}
\begin{align*}
  I_{1, 2} & = \frac{4^{1}\frac{h}{2}(f(a) + f(b) + 2f(\frac{a + b}{2})) - h(f(a) + f(b))}{4^{1} - 1}\\
  & = \frac{h}{3}\left (2(f(a) + f(b) + 2f(\frac{a + b}{2})) - (f(a) + f(b)) \right)\\
  & = \frac{h}{3} \left( f(a) + 4f\left(\frac{a + b}{2}\right) + f(b) \right) = S(f)
\end{align*}

\subsection{Teil b}

\begin{proof}
  Sei $f = ax^{3} + bx^{2} + cx + d \in \mathbb{P}_{3}$.

  Man berechne $\int_{i}^{j} f(x) dx$.
  \begin{align*}
    S(f) & = \frac{j - i}{6}(f(i) + 4f(\frac{i + j}{2}) + f(j))\\
    & = \frac{j - i}{6}\left( ai^{3} + bi^{2} + ci + d + 4 \left( a\left( \frac{i + j}{2} \right)^{3} + b\left( \frac{i + j}{2} \right)^{2} + c\left( \frac{i + j}{2} \right) + d \right) + aj^{3} + bj^{2} + cj + d \right)\\
    & = \frac{j - i}{6}\left( ai^{3} + bi^{2} + ci + \left( \frac{a}{2} (i + j)^{3} + b (i + j)^{2} + 2c(i + j) \right) + aj^{3} + bj^{2} + cj + 6d \right)\\
    & = \frac{j - i}{6}\left( ai^{3} + bi^{2} + ci + (i + j)\left( \frac{a}{2}i^{2} + aij + \frac{a}{2}j^{2} + bi + bj + 2c \right) + aj^{3} + bj^{2} + cj + 6d \right)\\
    & = \frac{j - i}{6}\left( ai^{3} + bi^{2} + ci + \left( \frac{a}{2}i^{3} + ai^{2}j + \frac{a}{2}j^{2}i + bi^{2} + bji + 2ci \right) + \left( \frac{a}{2}i^{2}j + aij^{2} + \frac{a}{2}j^{3} + bij + bj^{2} + 2cj \right) + aj^{3} + bj^{2} + cj + 6d \right)\\
    & = \frac{j - i}{6}\left( \frac{3a}{2}i^{3} + 2bi^{2} + 3ci + \frac{3a}{2}i^{2}j + \frac{3a}{2}ij^{2} + 2bji + \frac{3a}{2}j^{3} + 2bj^{2} + 3cj + 6d \right)\\
    & = (j - i)\left( \frac{a}{4}i^{3} + \frac{1}{3}bi^{2} + \frac{1}{2}ci + \frac{a}{4}i^{2}j + \frac{a}{4}ij^{2} + \frac{1}{3}bji + \frac{a}{4}j^{3} + \frac{1}{3}bj^{2} + \frac{1}{2}cj + d \right)\\
    & = \left( \frac{a}{4}i^{3}j + \frac{1}{3}bi^{2}j + \frac{1}{2}cij + \frac{a}{4}i^{2}j^{2} + \frac{a}{4}ij^{3} + \frac{1}{3}bij^{2} + \frac{a}{4}j^{4} + \frac{1}{3}bj^{3} + \frac{1}{2}cj^{2} + dj \right) - \left( \frac{a}{4}i^{4} + \frac{1}{3}bi^{3} + \frac{1}{2}ci^{2} + \frac{a}{4}i^{3}j + \frac{a}{4}i^{2}j^{2} + \frac{1}{3}bi^{2}j + \frac{a}{4}ij^{3} + \frac{1}{3}bij^{2} + \frac{1}{2}cij + di \right)\\
    & = \frac{a}{4}(j^{4} - i^{4}) + \frac{b}{3}(j^{3} - i^{3}) + \frac{c}{2}(j^{2} - i^{2}) + d(j - i)\\
    & = \frac{a}{4}j^{4} + \frac{b}{3}j^{3} + \frac{c}{2}j^{2} + dj - \left( \frac{a}{4}i^{4} + \frac{b}{3}i^{3} + \frac{c}{2}i^{2} + di \right)\\
    & = \left[ \frac{a}{4}x^{4} + \frac{b}{3}x^{2} + \frac{c}{2}x^{2} + dx \right]_{i}^{j}\\
    & = \int_{i}^{j} ax^{3} + bx^{2} + cx + d dx\\
    & = \int_{i}^{j} f(x) dx
  \end{align*}
\end{proof}

\section{Aufgabe 22}

\end{document}