\documentclass[10pt,a4paper]{article}
\usepackage[utf8]{inputenc}
\usepackage[german]{babel}
\usepackage{mathrsfs}
\usepackage{amsmath}
\usepackage{amsfonts}
\usepackage{amssymb}
\usepackage{amsthm}
\usepackage[left=2cm,right=2cm,top=2cm,bottom=2cm]{geometry}

\begin{document}

\section{Aufgabe 27}

\begin{equation}
  m_{1} = 1, M_{1} = s
\end{equation}
\begin{equation}
  m_{2} = 1, M_{2} = \sqrt{2} \cdot s
\end{equation}

\section{Aufgabe 28}

\begin{equation}
  L_{1} = \begin{pmatrix}
    1 & 0 & 0 & 0\\
    -1 & 1 & 0 & 0\\
    -1 & 0 & 1 & 0\\
    -1 & 0 & 0 & 1
  \end{pmatrix}
\end{equation}
\begin{equation}
  R_{1} = \begin{pmatrix}
    1 & 2 & 3 & 4\\
    0 & 2 & 6 & 12\\
    0 & 6 & 24 & 60\\
    0 & 14 & 78 & 252
  \end{pmatrix}
\end{equation}
\begin{equation}
  L_{2} = \begin{pmatrix}
    1 & 0 & 0 & 0\\
    0 & 1 & 0 & 0\\
    0 & -3 & 1 & 0\\
    0 & -7 & 0 & 1
  \end{pmatrix}
\end{equation}
\begin{equation}
  R_{2} = \begin{pmatrix}
    1 & 2 & 3 & 4\\
    0 & 2 & 6 & 12\\
    0 & 0 & 6 & 24\\
    0 & 0 & 36 & 168
  \end{pmatrix}
\end{equation}
\begin{equation}
  L_{3} = \begin{pmatrix}
    1 & 0 & 0 & 0\\
    0 & 1 & 0 & 0\\
    0 & 0 & 1 & 0\\
    0 & 0 & -6 & 1
  \end{pmatrix}
\end{equation}
\begin{equation}
  R_{3} = \begin{pmatrix}
    1 & 2 & 3 & 4\\
    0 & 2 & 6 & 12\\
    0 & 0 & 6 & 24\\
    0 & 0 & 0 & 24
  \end{pmatrix}
\end{equation}
\begin{equation}
  R = \begin{pmatrix}
    1 & 2 & 3 & 4\\
    0 & 2 & 6 & 12\\
    0 & 0 & 6 & 24\\
    0 & 0 & 0 & 24
  \end{pmatrix}
\end{equation}
\begin{equation}
  L = \begin{pmatrix}
    1 & 0 & 0 & 0\\
    1 & 1 & 0 & 0\\
    1 & 3 & 1 & 0\\
    1 & 7 & 6 & 1
  \end{pmatrix}
\end{equation}
\begin{equation}
  Ly = b
  \Leftrightarrow
  L = \begin{pmatrix}
    1 & 0 & 0 & 0\\
    1 & 1 & 0 & 0\\
    1 & 3 & 1 & 0\\
    1 & 7 & 6 & 1
  \end{pmatrix}
  \cdot
  \begin{pmatrix}
    y_{1}\\y_{2}\\y_{3}\\y_{4}
  \end{pmatrix}
  =
  \begin{pmatrix}
    3\\1\\-15\\-107
  \end{pmatrix}
  \Leftrightarrow
  y = \begin{pmatrix}
    3\\-2\\-12\\-24
  \end{pmatrix}
\end{equation}
\begin{equation}
  Rx = y
  \Leftrightarrow
  \begin{pmatrix}
    1 & 2 & 3 & 4\\
    0 & 2 & 6 & 12\\
    0 & 0 & 6 & 24\\
    0 & 0 & 0 & 24
  \end{pmatrix}
  \cdot
  \begin{pmatrix}
    x_{1}\\x_{2}\\x_{3}\\x_{4}
  \end{pmatrix}
  =
  \begin{pmatrix}
    3\\-2\\-12\\-24
  \end{pmatrix}
  \Leftrightarrow
  x = \begin{pmatrix}
    3\\-1\\2\\-1
  \end{pmatrix}
\end{equation}

\section{Aufgabe 29}

\end{document}