\documentclass[10pt,a4paper]{article}
\usepackage[utf8]{inputenc}
\usepackage[german]{babel}
\usepackage{amsmath}
\usepackage{amsfonts}
\usepackage{amssymb}
\usepackage{amsthm}
\usepackage[left=2cm,right=2cm,top=2cm,bottom=2cm]{geometry}

\begin{document}

\section*{Übung 1}

\section*{Übung 2}

\section*{Übung 3}

\subsection*{Teil 1}

\begin{proof}
Sei $a \in A$.
\begin{equation}
1a = a1 \Rightarrow 1 \in Z(A)
\end{equation}

Seien $a, b \in Z(A)$ und $c \in A$.
\begin{equation}
abc = acb = cab \Rightarrow ab \in Z(A)
\end{equation}
\end{proof}

\subsection*{Teil 2}

\begin{proof}
\begin{equation}
1 \in A_{0} \Rightarrow 1 \in A_{+}
\end{equation}

Seien $a, b \in A_{+}$.
\begin{equation}
ab = \left( \sum_{n \ge 0} a_{2n} \right)\left( \sum_{n \ge 0} b_{2n} \right) = \sum_{m \ge 0} \sum_{n \ge 0} a_{2m}b_{2n} \Rightarrow a_{2m}b_{2n} \in A_{2(m + n)} \Rightarrow ab \in A_{+}
\end{equation}
\end{proof}

\subsection*{Teil 3}

\begin{proof}
Sei $a \in A_{+}$ und $a' \in A$.
\begin{equation}
•
\end{equation}
\end{proof}

\subsection*{Teil 4}

\begin{proof}
Sei $a \in A_{2n + 1}$.
\begin{equation}
a^{2} = aa = (-1)^{(2n + 1)^{2}} aa = (-1)^{4n^{2} + 4n + 1} aa = -aa = -a^{2}
\end{equation}

Für $Char(K) = 0$, folgt sofort $a^{2} = 0$.
Sei $Char(K) = n > 0$.
\end{proof}

\subsection*{Teil 5}

\section*{Übung 4}

\section*{Übung 5}

\subsection*{Teil 1}

\subsubsection*{Teil a}

\subsubsection*{Teil b}

\subsubsection*{Teil c}

\subsection*{Teil 2}

\end{document}